src/RiscvBitWidths32.v
@@ -1,3 +1,0 @@
-Require Import riscv.RiscvBitWidths.
-
-Instance RiscvBitWidths32: RiscvBitWidths := Bitwidth32.
