src/RiscvBitWidths64.v
@@ -1,3 +1,0 @@
-Require Import riscv.RiscvBitWidths.
-
-Instance RiscvBitWidths64: RiscvBitWidths := Bitwidth64.
