src/util/BitWidth32.v
@@ -1,0 +1,3 @@
+Require Import riscv.util.BitWidths.
+
+Instance BitWidth32: BitWidths := BW32.
