src/util/BitWidth64.v
@@ -1,0 +1,3 @@
+Require Import riscv.util.BitWidths.
+
+Instance BitWidth64: BitWidths := BW64.
